Splinter/BTree.i.dfy
@@ -1,0 +1,27 @@
+include "../lib/Base/total_order.i.dfy"
+include "IndirectionTable.i.dfy"
+include "AllocationTable.i.dfy"
+include "AllocationTableMachine.i.dfy"
+include "MsgSeq.i.dfy"
+include "SplinterTree.i.dfy"
+include "Message.s.dfy"
+include "Interp.s.dfy"
+
+abstract module BtreeModel {
+  type Key = Keys.Element
+  type Value
+
+
+  datatype NodeState = None | OnDisk; // Might need arguments ???
+
+  // Node in the btree
+  // A node can either contain a key-value mapping (LEAF) or a sequence of
+  // pivots to provide an ordering of the children
+  datatype Node =
+    | Leaf(linear keys: seq<Key>, values: seq<Value>, state: NodeState)
+    | Index(linear pivots: seq<Key>, children: lseq<Node>)
+
+
+
+
+}
