Splinter/SplinterTreeInvariants.i.dfy
@@ -1,0 +1,25 @@
+include "SplinterTreeInterp.i.dfy"
+
+// Sowmya -- there might be a lot of invariants for this part as opposed to the journal, so I decided to make another module for this
+// If this ends up being sparse, we can just refactor it into BetreeInterpMod or ProgramMachineMod
+// Module that contains Betree's invariants needed in the RefinementProof
+module SplinterTreeInvariantMod {
+  import opened SplinterTreeInterpMod
+  import opened Options
+  import opened MessageMod
+  import opened InterpMod
+  import opened DiskTypesMod
+  import opened AllocationMod
+  import opened MsgSeqMod
+  import IndirectionTableMod
+  import opened SplinterTreeMachineMod
+  import Nat_Order
+
+  // TODO; Might need to change this to table about both IM and IMStable
+  lemma StableFraming(v: Variables, cache0: CacheIfc.Variables, cache1: CacheIfc.Variables, sb:Superblock)
+    requires DiskViewsEquivalentForSet(cache0.dv, cache1.dv, IReads(v, cache0, sb))
+    ensures IMStable(cache0, sb) == IMStable(cache1, sb)
+  {
+  }
+
+}
